A bunch of changes
File structure changes, context changes, more lemmas, etc.

src/semantic_rules_inter.v
@@ -1,10 +1,8 @@
 Require Import DTDT.syntax.
-Require Import DTDT.big_step_eval.
-Import ListNotations.
+Require Import DTDT.big_step_eval_inter.
 From stdpp Require Export base.
 From stdpp Require Export strings.
 From stdpp Require Import stringmap.
-
 
 (* --- Selfification rule ------------------------------------------------------ *)
 
@@ -50,8 +48,8 @@ Fixpoint self (type : i_ty) (term : i_expr) : i_ty :=
   | x => x
   end.
 
-Compute self (TBase BNat) (EVar ("x"%string)).
-Compute self (TArr (TBase BNat) (TArr (TBase BNat) (TBase BNat))) (EVar ("+"%string)).
+(* Compute self (TBase BNat) (EVar ("x"%string)).
+Compute self (TArr (TBase BNat) (TArr (TBase BNat) (TBase BNat))) (EVar ("+"%string)). *)
 
 
 (* --- Pure term validation ------------------------------------------------------ *)
@@ -80,196 +78,208 @@ Definition essential_type_is_base_type (type : i_ty) : bool :=
 Notation "β[ t ]" := (essential_type_is_base_type t) (at level 10).
 
 Inductive has_type_pure
-  ( Γ : var_context)
-  (Φ : const_context)
+  ( Γ : ctx)
   : i_expr -> i_ty -> Prop :=
   | PVar :
-    forall x τb,
-      Γ[ x ] Γ = Some τb ->
+    forall x τb e,
+      Γ !!₁ x = Some (τb, e) ->
       β[ τb ] ->
-      has_type_pure Γ Φ (EVar x) τb
+      has_type_pure Γ (EVar x) τb
   | PNat :
     forall n,
-      has_type_pure Γ Φ (ENat n) (TBase BNat)
+      has_type_pure Γ (ENat n) (TBase BNat)
   | PBool :
     forall b,
-      has_type_pure Γ Φ (EBool b) (TBase BBool)
+      has_type_pure Γ (EBool b) (TBase BBool)
   | PString :
     forall s,
-      has_type_pure Γ Φ (EString s) (TBase BString)
+      has_type_pure Γ (EString s) (TBase BString)
   | PUnit :
     forall u,
-      has_type_pure Γ Φ (EUnit u) (TBase BUnit)
+      has_type_pure Γ (EUnit u) (TBase BUnit)
   | PConst :
-    forall c τ,
-      Φ[ c ] Φ = Some τ ->
+    forall c τ e,
+      Γ !!₂ c = Some (τ, e) ->
       is_simple_type τ ->
-      has_type_pure Γ Φ (EConst c) τ
+      has_type_pure Γ (EConst c) τ
   | PApp :
     forall e₁ e₂ τ₁ τ₂,
       β[ τ₁ ] ->
-      has_type_pure Γ Φ e₁ (TArr τ₁ τ₂) ->
-      has_type_pure Γ Φ e₂ τ₁ ->
-      has_type_pure Γ Φ (EApp e₁ e₂) τ₂
+      has_type_pure Γ e₁ (TArr τ₁ τ₂) ->
+      has_type_pure Γ e₂ τ₁ ->
+      has_type_pure Γ (EApp e₁ e₂) τ₂
   | PNot :
     forall b,
-      has_type_pure Γ Φ b (TBase BBool) ->
-      has_type_pure Γ Φ (ENot b) (TBase BBool)
+      has_type_pure Γ b (TBase BBool) ->
+      has_type_pure Γ (ENot b) (TBase BBool)
   | PImp :
     forall b₁ b₂,
-      has_type_pure Γ Φ b₁ (TBase BBool) ->
-      has_type_pure Γ Φ b₂ (TBase BBool) ->
-      has_type_pure Γ Φ (EImp b₁ b₂) (TBase BBool)
+      has_type_pure Γ b₁ (TBase BBool) ->
+      has_type_pure Γ b₂ (TBase BBool) ->
+      has_type_pure Γ (EImp b₁ b₂) (TBase BBool)
   | PAnd :
     forall b₁ b₂,
-      has_type_pure Γ Φ b₁ (TBase BBool) ->
-      has_type_pure Γ Φ b₂ (TBase BBool) ->
-      has_type_pure Γ Φ (EAnd b₁ b₂) (TBase BBool)
+      has_type_pure Γ b₁ (TBase BBool) ->
+      has_type_pure Γ b₂ (TBase BBool) ->
+      has_type_pure Γ (EAnd b₁ b₂) (TBase BBool)
   | POr :
     forall b₁ b₂,
-      has_type_pure Γ Φ b₁ (TBase BBool) ->
-      has_type_pure Γ Φ b₂ (TBase BBool) ->
-      has_type_pure Γ Φ (EOr b₁ b₂) (TBase BBool)
+      has_type_pure Γ b₁ (TBase BBool) ->
+      has_type_pure Γ b₂ (TBase BBool) ->
+      has_type_pure Γ (EOr b₁ b₂) (TBase BBool)
   | PPlus :
     forall n₁ n₂,
-      has_type_pure Γ Φ n₁ (TBase BNat) ->
-      has_type_pure Γ Φ n₂ (TBase BNat) ->
-      has_type_pure Γ Φ (EPlus n₁ n₂) (TBase BNat).
+      has_type_pure Γ n₁ (TBase BNat) ->
+      has_type_pure Γ n₂ (TBase BNat) ->
+      has_type_pure Γ (EPlus n₁ n₂) (TBase BNat).
+
+Lemma const_lookup_add Γ f τ e :
+  (Γ ,,c f ↦ (τ, e)) !!₂ f = Some (τ,e).
+Proof.
+  unfold const_ctx_lookup.
+  unfold ctx_add_const. cbn.
+  apply lookup_insert.
+Qed.
+
+Lemma var_lookup_add Γ x τ e :
+  (Γ ,,v x ↦ (τ, e)) !!₁ x = Some (τ,e).
+Proof.
+  unfold var_ctx_lookup.
+  unfold ctx_add_var. cbn.
+  apply lookup_insert.
+Qed.
 
 Lemma pure_plus_app_nat :
-  has_type_pure [( "n" , TBase BNat)] [( "+" , TArr (TBase BNat) (TArr (TBase BNat) (TBase BNat)))] (EApp (EConst "+"%string) (ENat 1)) (TArr (TBase BNat) (TBase BNat)).
-  Proof.
-  apply (PApp _ _ _ _ (TBase BNat) _).
-  - simpl. reflexivity.
-  - apply PConst.
-    + simpl. reflexivity.
-    + simpl. reflexivity.
-  - apply PNat.
-  Qed.
+  has_type_pure ((ctx_add_const empty_ctx "+" (TArr (TBase BNat) (TArr (TBase BNat) (TBase BNat))) (EFix "" "n" (TBase BNat) (TArr (TBase BNat) (TBase BNat)) (EFix "" "m" (TBase BNat) (TBase BNat) (EPlus (EVar "n") (EVar "m"))))) ,,v "n" ↦ (TBase BNat, ENat 1)) (EApp (EConst "+"%string) (ENat 1)) (TArr (TBase BNat) (TBase BNat)).
+Proof.
+  apply PApp with (τ₁ := TBase BNat).
+  reflexivity.
+  eapply PConst.
+  apply const_lookup_add.
+  reflexivity.
+  apply PNat.
+Qed.
 
 Lemma pure_plus_app_var :
-  has_type_pure [( "n" , TBase BNat)] [( "+" , TArr (TBase BNat) (TArr (TBase BNat) (TBase BNat)))] (EApp (EConst "+"%string) (EVar "n")) (TArr (TBase BNat) (TBase BNat)).
-  Proof.
-  apply (PApp _ _ _ _ (TBase BNat) _).
-  - simpl. reflexivity.
-  - apply PConst.
-    + simpl. reflexivity.
-    + simpl. reflexivity.
-  - apply PVar.
-    + simpl. reflexivity.
-    + simpl. reflexivity.
-  Qed.
+  has_type_pure ((ctx_add_const empty_ctx "+" (TArr (TBase BNat) (TArr (TBase BNat) (TBase BNat))) (EFix "" "n" (TBase BNat) (TArr (TBase BNat) (TBase BNat)) (EFix "" "m" (TBase BNat) (TBase BNat) (EPlus (EVar "n") (EVar "m"))))) ,,v "n" ↦ (TBase BNat, ENat 1)) (EApp (EConst "+"%string) (EVar "n")) (TArr (TBase BNat) (TBase BNat)).
+Proof.
+  apply PApp with (τ₁ := TBase BNat).
+  reflexivity.
+  eapply PConst.
+  apply const_lookup_add.
+  reflexivity.
+  eapply PVar.
+  apply var_lookup_add.
+  reflexivity.
+Qed.
 
 (* --- Well-formed type checking ------------------------------------------------------ *)
 
 Inductive ty_valid
-  (Γ : var_context)
-  (Φ : const_context)
+  (Γ : ctx)
   : i_ty -> Prop :=
   | VBase :
     forall (τb : BaseT),
-      ty_valid Γ Φ (TBase τb)
+      ty_valid Γ (TBase τb)
   | VSet :
-    forall var (τb : BaseT) e,
-      has_type_pure ((var , TBase τb) :: Γ) Φ e (TBase BBool) ->
-      ty_valid Γ Φ (TSet var τb e)
+    forall var (τb : BaseT) e v,
+      has_type_pure (ctx_add_var Γ var (TBase τb) v) e (TBase BBool) ->
+      ty_valid Γ (TSet var τb e)
   | VFun :
     forall τ₁ τ₂,
-      ty_valid Γ Φ τ₁ ->
-      ty_valid Γ Φ τ₂ ->
-      ty_valid Γ Φ (TArr τ₁ τ₂)
+      ty_valid Γ τ₁ ->
+      ty_valid Γ τ₂ ->
+      ty_valid Γ (TArr τ₁ τ₂)
   | VFunDep :
-    forall var τ₁ τ₂,
-      ty_valid Γ Φ τ₁ ->
-      ty_valid ((var, τ₁) :: Γ) Φ τ₂ ->
-      ty_valid Γ Φ (TArrDep var τ₁ τ₂)
+    forall var τ₁ τ₂ v,
+      ty_valid Γ τ₁ ->
+      ty_valid (ctx_add_var Γ var τ₁ v) τ₂ ->
+      ty_valid Γ (TArrDep var τ₁ τ₂)
   | VPair :
     forall τ₁ τ₂,
-      ty_valid Γ Φ τ₁ ->
-      ty_valid Γ Φ τ₂ ->
-      ty_valid Γ Φ (TProd τ₁ τ₂)
+      ty_valid Γ τ₁ ->
+      ty_valid Γ τ₂ ->
+      ty_valid Γ (TProd τ₁ τ₂)
   | VRef :
     forall τ₁,
-      ty_valid Γ Φ τ₁ ->
-      ty_valid Γ Φ (TRef τ₁).
+      ty_valid Γ τ₁ ->
+      ty_valid Γ (TRef τ₁).
 
 (* --- Subtyping ---------------------------------------------------------------------- *)
 
 (* Should this be on surface level? In paper there's a rule for dereferation too *)
 Inductive subtype 
-  (Γ : var_context)
-  (Γv : varval_context)
-  (Φ : const_context)
-  (ι : fun_imp_list) :
+  (Γ : ctx) :
   i_ty -> i_ty -> Prop :=
   | SBase :
     forall b,
-      subtype Γ Γv Φ ι (TBase b) (TBase b)
+      subtype Γ (TBase b) (TBase b)
   | SSet :
     forall var τb e₁ e₂,
-      ty_valid Γ Φ (TSet var τb e₁) ->
-      ty_valid Γ Φ (TSet var τb e₂) ->
-      ∀ (c : (base_to_set τb)), eval ((var , TBase τb) :: Γ) ((var , make_expr τb c) :: Γv) Φ ι (EImp e₁ e₂) (EBool true) ->
-      subtype Γ Γv Φ ι (TSet var τb e₁) (TSet var τb e₂)
+      ty_valid Γ (TSet var τb e₁) ->
+      ty_valid Γ (TSet var τb e₂) ->
+      ∀ (c : (base_to_set τb)), eval (ctx_add_var Γ var (TBase τb) (make_expr τb c)) (EImp e₁ e₂) (EBool true) ->
+      subtype Γ (TSet var τb e₁) (TSet var τb e₂)
   | SSetBase :
     forall var τb e,
-      ty_valid Γ Φ (TSet var τb e) ->
-      subtype Γ Γv Φ ι (TSet var τb e) (TBase τb)
+      ty_valid Γ (TSet var τb e) ->
+      subtype Γ (TSet var τb e) (TBase τb)
   | SBaseSet :
     forall var τb e,
-      ty_valid Γ Φ (TSet var τb e) ->
-      ∀ (c : (base_to_set τb)), eval ((var , TBase τb) :: Γ) ((var , make_expr τb c) :: Γv) Φ ι e (EBool true) ->
-      subtype Γ Γv Φ ι (TBase τb) (TSet var τb e)
+      ty_valid Γ (TSet var τb e) ->
+      ∀ (c : (base_to_set τb)), eval (ctx_add_var Γ var (TBase τb) (make_expr τb c)) e (EBool true) ->
+      subtype Γ (TBase τb) (TSet var τb e)
   | SFun :
     forall τ₁ τ₁' τ₂ τ₂',
-      subtype Γ Γv Φ ι τ₁' τ₁ ->
-      subtype Γ Γv Φ ι τ₂ τ₂' ->
-      subtype Γ Γv Φ ι (TArr τ₁ τ₂) (TArr τ₁' τ₂')
+      subtype Γ τ₁' τ₁ ->
+      subtype Γ τ₂ τ₂' ->
+      subtype Γ (TArr τ₁ τ₂) (TArr τ₁' τ₂')
   | SFunDep :
-    forall var τ₁ τ₁' τ₂ τ₂',
-      subtype Γ Γv Φ ι τ₁' τ₁ ->
-      subtype ((var , τ₁') :: Γ) Γv Φ ι τ₂ τ₂' ->
-      subtype Γ Γv Φ ι (TArrDep var τ₁ τ₂) (TArrDep var τ₁' τ₂')
+    forall var τ₁ τ₁' τ₂ τ₂' v,
+      subtype Γ τ₁' τ₁ ->
+      subtype (ctx_add_var Γ var τ₁' v) τ₂ τ₂' ->
+      subtype Γ (TArrDep var τ₁ τ₂) (TArrDep var τ₁' τ₂')
   | SPair :
     forall τ₁ τ₁' τ₂ τ₂',
-      subtype Γ Γv Φ ι τ₁ τ₁' ->
-      subtype Γ Γv Φ ι τ₂ τ₂' ->
-      subtype Γ Γv Φ ι (TProd τ₁ τ₂) (TProd τ₁' τ₂')
+      subtype Γ τ₁ τ₁' ->
+      subtype Γ τ₂ τ₂' ->
+      subtype Γ (TProd τ₁ τ₂) (TProd τ₁' τ₂')
   | SRef :
     forall τ τ',
-      subtype Γ Γv Φ ι τ τ' ->
-      subtype Γ Γv Φ ι τ' τ ->
-      subtype Γ Γv Φ ι (TRef τ) (TRef τ').
+      subtype Γ τ τ' ->
+      subtype Γ τ' τ ->
+      subtype Γ (TRef τ) (TRef τ').
 
-Lemma set_sub_test : forall Γ Γv Φ ι, subtype Γ Γv Φ ι (TSet "x" BBool (ENot (EVar "x"))) (TSet "x" BBool (EBool true)).
+Lemma set_sub_test : forall Γ, subtype Γ (TSet "x" BBool (ENot (EVar "x"))) (TSet "x" BBool (EBool true)).
 Proof.
 intros.
 eapply SSet.
-apply VSet.
+apply VSet with (v := EBool true).
 apply PNot.
-apply PVar.
-simpl. reflexivity.
-simpl. reflexivity.
-apply VSet.
+apply PVar with (e := EBool true).
+unfold var_ctx_lookup.
+apply var_lookup_add.
+reflexivity.
+apply VSet with (v := ENat 1).
 apply PBool.
 simpl.
 apply eval_imp with (e₁ := ENot (EVar "x")) (e₂ := EBool true) (b₁ := true) (b₂ := true).
 apply eval_not with (b := false).
 eapply eval_var.
-simpl; reflexivity.
-simpl; reflexivity.
+unfold var_ctx_lookup.
+apply var_lookup_add.
 apply eval_bool.
 Qed.
 
 (* two equivalent sets *)
-Lemma set_sub_test_without_var_use : forall Γ Γv Φ ι, subtype Γ Γv Φ ι (TSet "x" BBool (ENot (EBool false))) (TSet "x" BBool (EBool true)).
+Lemma set_sub_test_without_var_use : forall Γ, subtype Γ (TSet "x" BBool (ENot (EBool false))) (TSet "x" BBool (EBool true)).
 Proof.
 intros.
 apply SSet with (c := true).
-apply VSet.
+apply VSet with (v := ENat 0).
 apply PNot.
 apply PBool.
-apply VSet.
+apply VSet with (v := ENat 0).
 apply PBool.
 simpl.
 apply eval_imp with (e₁ := ENot (EBool false)) (e₂ := EBool true) (b₁ := true) (b₂ := true).
@@ -279,14 +289,14 @@ apply eval_bool.
 Qed.
 
 (* actual subsets *)
-Lemma set_sub_test_without_var_use2 : forall Γ Γv Φ ι, subtype Γ Γv Φ ι (TSet "x" BBool (ENot (EBool true))) (TSet "x" BBool (EBool true)).
+Lemma set_sub_test_without_var_use2 : forall Γ, subtype Γ (TSet "x" BBool (ENot (EBool true))) (TSet "x" BBool (EBool true)).
 Proof.
 intros.
 apply SSet with (c := true).
-apply VSet.
+apply VSet with (v := EBool false).
 apply PNot.
 apply PBool.
-apply VSet.
+apply VSet with (v := EBool false).
 apply PBool.
 apply eval_imp with (e₁ := ENot (EBool true)) (e₂ := EBool true) (b₁ := false) (b₂ := true).
 apply eval_not with (e := EBool true) (b := true).
@@ -294,22 +304,22 @@ apply eval_bool.
 apply eval_bool.
 Qed.
 
-Lemma base_sub_set_test : forall Γ Γv Φ ι, subtype Γ Γv Φ ι (TBase BBool) (TSet "x" BBool (EOr (EBool true) (EVar "x"))).
+Lemma base_sub_set_test : forall Γ, subtype Γ (TBase BBool) (TSet "x" BBool (EOr (EBool true) (EVar "x"))).
 Proof.
 intros.
 eapply SBaseSet.
-apply VSet.
+apply VSet with (v := ENat 2).
 apply POr.
 apply PBool.
-apply PVar.
-simpl; reflexivity.
-simpl; reflexivity.
-simpl.
+apply PVar with (e := ENat 2).
+unfold var_ctx_lookup.
+apply var_lookup_add.
+reflexivity.
 apply eval_or with (b₁ := true) (b₂ := false).
 apply eval_bool.
 eapply eval_var.
-simpl; reflexivity.
-simpl; reflexivity.
+unfold var_ctx_lookup.
+apply var_lookup_add.
 Qed.
 
 (* ------------------------------------------------------------------------- *)
@@ -360,68 +370,82 @@ Fixpoint ty_subst (x : string) (s : i_expr) (τ : i_ty) : i_ty :=
 (* --- Type rules for the internal language ------------------------------------------- *)
 
 Inductive has_type
-  ( Γ : var_context)
-  (Γv : varval_context)
-  (Φ : const_context)
-  (ι : fun_imp_list)
+  ( Γ : ctx)
   : i_expr -> i_ty -> Prop :=
+  | TString :
+    forall s,
+      has_type Γ (EString s) (TBase BString)
+  | TNat :
+    forall n,
+      has_type Γ (ENat n) (TBase BNat)
+  | TBool :
+    forall b,
+      has_type Γ (EBool b) (TBase BBool)
+  | TUnit :
+    forall u,
+      has_type Γ (EUnit u) (TBase BUnit)
   | TConst :
-    forall c τ,
-      Φ[ c ] Φ = Some τ ->
-      has_type Γ Γv Φ ι (EConst c) τ
+    forall c τ e,
+      Γ !!₂ c = Some (τ, e) ->
+      has_type Γ (EConst c) τ
   | TVar :
-    forall v τ,
-      Γ[ v ] Γ = Some τ ->
-      has_type Γ Γv Φ ι (EVar v) τ
+    forall v τ e,
+      Γ !!₁ v = Some (τ, e) ->
+      has_type Γ (EVar v) τ
   | TFail :
     forall τ,
-      ty_valid Γ Φ τ ->
-      has_type Γ Γv Φ ι EFail τ
+      ty_valid Γ τ ->
+      has_type Γ EFail τ
   | TFun :
-    forall f x τ₁ τ₂ e,
-      ty_valid Γ Φ (TArrDep x τ₁ τ₂) ->
-      has_type Γ Γv ((f , (TArrDep x τ₁ τ₂)) :: Φ) ι e τ₂ ->
-      has_type Γ Γv Φ ι (EFix f x τ₁ τ₂ e) (TArrDep x τ₁ τ₂)
+    forall f x τ₁ τ₂ e exp,
+      ty_valid Γ (TArrDep x τ₁ τ₂) ->
+      has_type (ctx_add_const Γ f (TArrDep x τ₁ τ₂) exp) e τ₂ ->
+      has_type Γ (EFix f x τ₁ τ₂ e) (TArrDep x τ₁ τ₂)
   | TAppPure :
     forall e₁ e₂ x τ₁ τ₂,
-      has_type Γ Γv Φ ι e₂ τ₁ ->
-      (forall τ₃, has_type_pure Γ Φ e₂ τ₃) ->
-      has_type Γ Γv Φ ι e₁ (TArrDep x τ₁ τ₂) ->
-      has_type Γ Γv Φ ι (expr_subst x e₂ e₁) τ₂ ->
-      has_type Γ Γv Φ ι (EApp e₁ e₂) τ₂
+      has_type Γ e₂ τ₁ ->
+      (forall τ₃, has_type_pure Γ e₂ τ₃) ->
+      has_type Γ e₁ (TArrDep x τ₁ τ₂) ->
+      has_type Γ (expr_subst x e₂ e₁) τ₂ ->
+      has_type Γ (EApp e₁ e₂) τ₂
   | TAppImPure :
     forall e₁ e₂ τ₁ τ₂,
-      has_type Γ Γv Φ ι e₂ τ₁ ->
-      has_type Γ Γv Φ ι e₁ (TArr τ₁ τ₂) ->
-      has_type Γ Γv Φ ι (EApp e₁ e₂) τ₂
+      has_type Γ e₂ τ₁ ->
+      has_type Γ e₁ (TArr τ₁ τ₂) ->
+      has_type Γ (EApp e₁ e₂) τ₂
+  | TPlus :
+    forall e₁ e₂,
+      has_type Γ e₁ (TBase BNat) ->
+      has_type Γ e₂ (TBase BNat) ->
+      has_type Γ (EPlus e₁ e₂) (TBase BNat)
   | TPair :
     forall e₁ e₂ τ₁ τ₂,
-      has_type Γ Γv Φ ι e₁ τ₁ ->
-      has_type Γ Γv Φ ι e₂ τ₂ ->
-      has_type Γ Γv Φ ι (EPair e₁ e₂) (TProd τ₁ τ₂)
+      has_type Γ e₁ τ₁ ->
+      has_type Γ e₂ τ₂ ->
+      has_type Γ (EPair e₁ e₂) (TProd τ₁ τ₂)
   | TFst :
     forall e τ₁ τ₂,
-      has_type Γ Γv Φ ι e (TProd τ₁ τ₂) ->
-      has_type Γ Γv Φ ι (EFst e) τ₁
+      has_type Γ e (TProd τ₁ τ₂) ->
+      has_type Γ (EFst e) τ₁
   | TSnd :
     forall e τ₁ τ₂,
-      has_type Γ Γv Φ ι e (TProd τ₁ τ₂) ->
-      has_type Γ Γv Φ ι (ESnd e) τ₂
+      has_type Γ e (TProd τ₁ τ₂) ->
+      has_type Γ (ESnd e) τ₂
   | TIf :
     forall e e₁ e₂ τ u,
-      has_type_pure Γ Φ e (TBase BBool) ->
-      has_type ((u , TBase BBool) :: Γ) ((u , e) :: Γv) Φ ι e₁ τ ->
-      has_type ((u , TBase BBool) :: Γ) ((u , ENot e) :: Γv) Φ ι e₂ τ ->
-      has_type Γ Γv Φ ι (EIf e e₁ e₂) τ
+      has_type_pure Γ e (TBase BBool) ->
+      has_type (ctx_add_var Γ u (TBase BBool) e) e₁ τ ->
+      has_type (ctx_add_var Γ u (TBase BBool) (ENot e)) e₂ τ ->
+      has_type Γ (EIf e e₁ e₂) τ
   | TSelf :
     forall e τ,
-      has_type Γ Γv Φ ι e τ ->
-      (forall τ₁, has_type_pure Γ Φ e τ₁) ->
-      has_type Γ Γv Φ ι e (self τ e)
+      has_type Γ e τ ->
+      (forall τ₁, has_type_pure Γ e τ₁) ->
+      has_type Γ e (self τ e)
   | TSub :
     forall e τ τ',
-      has_type Γ Γv Φ ι e τ' ->
-      subtype Γ Γv Φ ι τ' τ ->
-      has_type Γ Γv Φ ι e τ.
+      has_type Γ e τ' ->
+      subtype Γ τ' τ ->
+      has_type Γ e τ.
 
 
