src/semantic_lemmas_inter.v
@@ -1,0 +1,173 @@
+Require Import DTDT.syntax.
+Require Import DTDT.big_step_eval_inter.
+Require Import DTDT.semantic_rules_inter.
+
+Definition add_ctx (Γ₁ Γ₂ : ctx) : ctx := ((Γ₂ ▷vars) ∪ (Γ₁ ▷vars), (Γ₂ ▷consts) ∪ (Γ₁ ▷consts)).
+
+(* --- Lemmas ------------------------------------------------------------ *)
+
+Lemma lookup_lemma_const : forall Γ₁ Γ₂ Γ₃ c τ e,
+  ((add_ctx Γ₂ Γ₁) !!₂ c) = (Some (τ, e)) ->
+  ((add_ctx (add_ctx Γ₃ Γ₂) Γ₁) !!₂ c) = (Some (τ, e)).
+Proof.
+  intros.
+  unfold add_ctx, const_ctx_lookup in *. cbn in *.
+  destruct ((snd Γ₁) !! c) eqn:H2.
+  - (* c is in Γ2 *)
+    apply (lookup_union_Some_l (Γ₁.2) _ c _).
+    rewrite <- H.
+    rewrite H2 at 1.
+    symmetry.
+    apply (lookup_union_Some_l (Γ₁.2) _ c _).
+    exact H2.
+  - (* c not in Γ2 *)
+    pose proof (lookup_union_r (Γ₁.2) (Γ₂.2) c H2).
+    pose proof (lookup_union_r (Γ₁.2) ((Γ₂.2) ∪ (Γ₃.2)) c H2).
+    rewrite H1 at 1.
+    rewrite H0 in H at 1.
+    apply (lookup_union_Some_l (Γ₂.2) _ c _).
+    exact H.
+Qed.
+
+Lemma lookup_lemma_var : forall Γ₁ Γ₂ Γ₃ c τ e,
+  ((add_ctx Γ₂ Γ₁) !!₁ c) = (Some (τ, e)) ->
+  ((add_ctx (add_ctx Γ₃ Γ₂) Γ₁) !!₁ c) = (Some (τ, e)).
+Proof.
+  intros.
+  unfold add_ctx, var_ctx_lookup in *. cbn in *.
+  destruct ((fst Γ₁) !! c) eqn:H2.
+  - (* c is in Γ2 *)
+    apply (lookup_union_Some_l (Γ₁.1) _ c _).
+    rewrite <- H.
+    rewrite H2 at 1.
+    symmetry.
+    apply (lookup_union_Some_l (Γ₁.1) _ c _).
+    exact H2.
+  - (* c not in Γ2 *)
+    pose proof (lookup_union_r (Γ₁.1) (Γ₂.1) c H2).
+    pose proof (lookup_union_r (Γ₁.1) ((Γ₂.1) ∪ (Γ₃.1)) c H2).
+    rewrite H1 at 1.
+    rewrite H0 in H at 1.
+    apply (lookup_union_Some_l (Γ₂.1) _ c _).
+    exact H.
+Qed.
+
+Lemma lookup_lemma_var_add : forall Γ₁ Γ₂ Γ₃ c τ e v type exp,
+  ((ctx_add_var (add_ctx Γ₂ Γ₁) v type exp) !!₁ c) = (Some (τ, e)) ->
+  ((ctx_add_var (add_ctx (add_ctx Γ₃ Γ₂) Γ₁) v type exp) !!₁ c) = (Some (τ, e)).
+Proof.
+  intros.
+  unfold ctx_add_var, add_ctx, var_ctx_lookup in *. simpl in *.
+  Search union.
+  pose proof (insert_union_singleton_l ((Γ₁.1) ∪ ((Γ₂.1) ∪ (Γ₃.1)))).
+  rewrite (H0 v (type, exp)) at 1.
+  Print lookup_singleton.
+  destruct (({[ v := (type,exp) ]} : gmap string (i_ty * i_expr)) !! c) eqn:Hlookup.
+  - apply (lookup_union_Some_l ({[ v := (type,exp) ]} : gmap string (i_ty * i_expr)) _ c _).
+    rewrite <- H.
+    symmetry.
+    pose proof (insert_union_singleton_l ((Γ₁.1) ∪ (Γ₂.1))).
+    rewrite (H1 v (type, exp)) at 1.
+    rewrite Hlookup.
+    apply (lookup_union_Some_l ({[ v := (type,exp) ]} : gmap string (i_ty * i_expr)) _ c _).
+    exact Hlookup.
+  - pose proof (lookup_union_r ({[ v := (type,exp) ]} : gmap string (i_ty * i_expr)) ((Γ₁.1) ∪ ((Γ₂.1) ∪ (Γ₃.1))) c Hlookup).
+    rewrite H1 at 1.
+    pose proof (lookup_union_r ({[ v := (type,exp) ]} : gmap string (i_ty * i_expr)) ((Γ₁.1) ∪ (Γ₂.1)) c Hlookup).
+    pose proof (insert_union_singleton_l ((Γ₁.1) ∪ (Γ₂.1))).
+    rewrite (H3 v (type, exp)) in H at 1.
+    rewrite H2 in H at 1.
+    apply lookup_lemma_var. exact H.
+Qed.
+
+Lemma weakening_has_type_pure :
+  forall Γ₁ Γ₂ Γ₃ e τ,
+    has_type_pure (add_ctx Γ₂ Γ₁) e τ ->
+    has_type_pure (add_ctx (add_ctx Γ₃ Γ₂) Γ₁) e τ.
+Proof.
+  intros.
+  revert Γ₁ Γ₂ Γ₃ τ H.
+  induction e; intros; inversion H.
+  apply PString.
+  apply PBool.
+  apply PNat.
+  apply PUnit.
+  eapply PConst. apply lookup_lemma_const. exact H1. exact H2.
+  eapply PVar. apply lookup_lemma_var. exact H1. exact H2.
+  eapply PApp. exact H2. apply IHe1. exact H3. apply IHe2. exact H5.
+  apply PPlus. apply IHe1. exact H2. apply IHe2. exact H4.
+  apply PNot. apply IHe. exact H1.
+  apply PAnd. apply IHe1. assumption. apply IHe2. assumption.
+  apply POr. apply IHe1. assumption. apply IHe2. assumption.
+  apply PImp. apply IHe1. assumption. apply IHe2. assumption.
+Qed.
+
+Lemma weakening_has_type_pure_add :
+  forall Γ₁ Γ₂ Γ₃ var exp type e τ,
+    has_type_pure (ctx_add_var (add_ctx Γ₂ Γ₁) var exp type) e τ ->
+    has_type_pure (ctx_add_var (add_ctx (add_ctx Γ₃ Γ₂) Γ₁) var exp type) e τ.
+Proof.
+  intros.
+  revert Γ₁ Γ₂ Γ₃ τ H.
+  induction e; intros; inversion H; subst.
+  apply PString.
+  apply PBool.
+  apply PNat.
+  apply PUnit.
+  eapply PConst. apply lookup_lemma_const. exact H1. exact H2.
+  eapply PVar. apply lookup_lemma_var_add. exact H1. exact H2.
+  eapply PApp. exact H2. apply IHe1. exact H3. apply IHe2. exact H5.
+  apply PPlus. apply IHe1. exact H2. apply IHe2. exact H4.
+  apply PNot. apply IHe. exact H1.
+  apply PAnd. apply IHe1. assumption. apply IHe2. assumption.
+  apply POr. apply IHe1. assumption. apply IHe2. assumption.
+  apply PImp. apply IHe1. assumption. apply IHe2. assumption.
+Qed.
+
+Lemma weakening_ty_valid :
+  forall Γ₁ Γ₂ Γ₃ τ,
+    ty_valid (add_ctx Γ₂ Γ₁) τ ->
+    ty_valid (add_ctx (add_ctx Γ₃ Γ₂) Γ₁) τ.
+Proof.
+  intros.
+  revert Γ₁ Γ₂ Γ₃ H.
+  induction τ; intros.
+  apply VBase.
+  eapply VSet.
+  apply (weakening_has_type_pure_add Γ₁ Γ₂ Γ₃ s (TBase b) _ i (TBase BBool)).
+  admit.
+  apply VFun. apply IHτ1. inversion H. assumption. apply IHτ2. inversion H. assumption.
+  eapply VFunDep. apply IHτ1. inversion H. assumption. admit.
+  apply VPair. inversion H. apply IHτ1. assumption. inversion H. apply IHτ2. assumption.
+  apply VRef. inversion H. apply IHτ. assumption.
+Admitted.
+
+
+Lemma weakening :
+  forall Γ₁ Γ₂ Γ₃ e τ,
+    has_type (add_ctx Γ₂ Γ₁) e τ ->
+    has_type (add_ctx (add_ctx Γ₃ Γ₂) Γ₁) e τ.
+Proof.
+intros.
+simpl.
+inversion H.
+apply TString.
+apply TNat.
+apply TBool.
+apply TUnit.
+eapply TConst.
+apply lookup_lemma_const. exact H0.
+eapply TVar.
+apply lookup_lemma_var. exact H0.
+apply TFail. apply weakening_ty_valid. assumption.
+eapply TFun. apply weakening_ty_valid. assumption. admit.
+eapply TAppPure. admit. admit. admit. admit.
+eapply TAppImPure. admit. admit.
+apply TPlus. admit. admit. admit.
+eapply TFst. admit.
+eapply TSnd. admit.
+eapply TIf. admit. admit. admit.
+apply TSelf. admit. admit.
+eapply TSub. admit. admit.
+Admitted.
+
