src/semantic_rules_surf.v
@@ -1,0 +1,164 @@
+Require Import DTDT.syntax.
+Require Import DTDT.big_step_eval_inter.
+Require Import DTDT.semantic_rules_inter.
+
+(* --- Pure term validation - surface language -------------------------------------------- *)
+
+Fixpoint is_simple_type_surf (type : ty) : bool :=
+  match type with
+  | TyBase _ => true
+  | TyArr t1 t2 => is_simple_type_surf t1 && is_simple_type_surf t2
+  | TyProd t1 t2 => is_simple_type_surf t1 && is_simple_type_surf t2
+  | _ => false
+  end.
+
+Definition essential_type_is_base_type_surf (type : ty) : bool :=
+  match type with
+  | TyBase _ => true
+  | TySet _ _ _ => true
+  | _ => false
+  end.
+Notation "βs[ t ]" := (essential_type_is_base_type_surf t) (at level 10).
+
+Inductive has_type_pure_surf
+  ( Γ : ctx_surf)
+  : expr -> ty -> Prop :=
+  | PVarS :
+    forall x τb v,
+      Γ !!₁ₛ x = Some (τb, v) ->
+      βs[ τb ] ->
+      has_type_pure_surf Γ (ExVar x) τb
+  | PNatS :
+    forall n,
+      has_type_pure_surf Γ (ExNat n) (TyBase BNat)
+  | PBoolS :
+    forall b,
+      has_type_pure_surf Γ (ExBool b) (TyBase BBool)
+  | PStringS :
+    forall s,
+      has_type_pure_surf Γ (ExString s) (TyBase BString)
+  | PUnitS :
+    forall u,
+      has_type_pure_surf Γ (ExUnit u) (TyBase BUnit)
+  | PConstS :
+    forall c τ v,
+      Γ !!₂ₛ c = Some (τ, v) ->
+      is_simple_type_surf τ ->
+      has_type_pure_surf Γ (ExConst c) τ
+  | PAppS :
+    forall e₁ e₂ τ₁ τ₂,
+      βs[ τ₁ ] ->
+      has_type_pure_surf Γ e₁ (TyArr τ₁ τ₂) ->
+      has_type_pure_surf Γ e₂ τ₁ ->
+      has_type_pure_surf Γ (ExApp e₁ e₂) τ₂
+  | PNotS :
+    forall b,
+      has_type_pure_surf Γ b (TyBase BBool) ->
+      has_type_pure_surf Γ (ExNot b) (TyBase BBool)
+  | PImpS :
+    forall b₁ b₂,
+      has_type_pure_surf Γ b₁ (TyBase BBool) ->
+      has_type_pure_surf Γ b₂ (TyBase BBool) ->
+      has_type_pure_surf Γ (ExImp b₁ b₂) (TyBase BBool)
+  | PAndS :
+    forall b₁ b₂,
+      has_type_pure_surf Γ b₁ (TyBase BBool) ->
+      has_type_pure_surf Γ b₂ (TyBase BBool) ->
+      has_type_pure_surf Γ (ExAnd b₁ b₂) (TyBase BBool)
+  | POrS :
+    forall b₁ b₂,
+      has_type_pure_surf Γ b₁ (TyBase BBool) ->
+      has_type_pure_surf Γ b₂ (TyBase BBool) ->
+      has_type_pure_surf Γ (ExOr b₁ b₂) (TyBase BBool)
+  | PPlusS :
+    forall n₁ n₂,
+      has_type_pure_surf Γ n₁ (TyBase BNat) ->
+      has_type_pure_surf Γ n₂ (TyBase BNat) ->
+      has_type_pure_surf Γ (ExPlus n₁ n₂) (TyBase BNat).
+
+(* --- Type wellformedness for surface language -----------------------------*)
+
+Inductive ty_valid_surf
+  (Γ : ctx_surf)
+  : ty -> Prop :=
+  | VBaseS :
+    forall (τb : BaseT),
+      ty_valid_surf Γ (TyBase τb)
+  | VSetS :
+    forall var (τb : BaseT) e v,
+      has_type_pure_surf (ctx_add_var_surf Γ var (TyBase τb) v) e (TyBase BBool) ->
+      ty_valid_surf Γ (TySet var τb e)
+  | VFunS :
+    forall τ₁ τ₂,
+      ty_valid_surf Γ τ₁ ->
+      ty_valid_surf Γ τ₂ ->
+      ty_valid_surf Γ (TyArr τ₁ τ₂)
+  | VFunDepS :
+    forall var τ₁ τ₂ v,
+      ty_valid_surf Γ τ₁ ->
+      ty_valid_surf (ctx_add_var_surf Γ var τ₁ v) τ₂ ->
+      ty_valid_surf Γ (TyArrDep var τ₁ τ₂)
+  | VPairS :
+    forall τ₁ τ₂,
+      ty_valid_surf Γ τ₁ ->
+      ty_valid_surf Γ τ₂ ->
+      ty_valid_surf Γ (TyProd τ₁ τ₂)
+  | VRefS :
+    forall τ₁,
+      ty_valid_surf Γ τ₁ ->
+      ty_valid_surf Γ (TyRef τ₁)
+  | VDeRefS :
+    forall τ₁,
+      ty_valid_surf Γ τ₁ ->
+      ty_valid_surf Γ (TyDeRef τ₁).
+
+(* --- Substitution for surface language ----------------------------------- *)
+
+Fixpoint expr_subst_surf (x : string) (s : expr) (e : expr) : expr :=
+  match e with
+  | ExVar y =>
+      if String.eqb x y then s else ExVar y
+  | ExConst c => ExConst c
+  | ExString v => ExString v
+  | ExBool b => ExBool b
+  | ExNat n => ExNat n
+  | ExUnit u => ExUnit u
+  | ExFix f y τ1 τ2 body =>
+      if String.eqb f x || String.eqb y x then ExFix f y τ1 τ2 body
+      else ExFix f y τ1 τ2 (expr_subst_surf x s body)
+  | ExApp e1 e2 => ExApp (expr_subst_surf x s e1) (expr_subst_surf x s e2)
+  | ExPlus e1 e2 => ExPlus (expr_subst_surf x s e1) (expr_subst_surf x s e2)
+  | ExPair e1 e2 => ExPair (expr_subst_surf x s e1) (expr_subst_surf x s e2)
+  | ExFst e1 => ExFst (expr_subst_surf x s e1)
+  | ExSnd e1 => ExSnd (expr_subst_surf x s e1)
+  | ExIf e1 e2 e3 => ExIf (expr_subst_surf x s e1) (expr_subst_surf x s e2) (expr_subst_surf x s e3)
+  | ExNot e1 => ExNot (expr_subst_surf x s e1)
+  | ExAnd e1 e2 => ExAnd (expr_subst_surf x s e1) (expr_subst_surf x s e2)
+  | ExOr e1 e2 => ExOr (expr_subst_surf x s e1) (expr_subst_surf x s e2)
+  | ExImp e1 e2 => ExImp (expr_subst_surf x s e1) (expr_subst_surf x s e2)
+  | ExEq e1 e2 => ExEq (expr_subst_surf x s e1) (expr_subst_surf x s e2)
+  | ExNewRef τ e1 => ExNewRef τ (expr_subst_surf x s e1)
+  | ExGet e1 => ExGet (expr_subst_surf x s e1)
+  | ExSet e1 e2 => ExSet (expr_subst_surf x s e1) (expr_subst_surf x s e2)
+  | ExDeRef e1 => ExDeRef (expr_subst_surf x s e1)
+  | ExGetDep e1 => ExGetDep (expr_subst_surf x s e1)
+  | ExSetDep e1 e2 => ExSetDep (expr_subst_surf x s e1) (expr_subst_surf x s e2)
+  | EAssert e τ => EAssert (expr_subst_surf x s e) τ
+  | ESimple e => ESimple (expr_subst_surf x s e)
+  | EDep e => EDep (expr_subst_surf x s e)
+  end.
+
+Fixpoint ty_subst_surf (x : string) (s : expr) (τ : ty) : ty :=
+  match τ with
+  | TyBase b => TyBase b
+  | TySet y b pred =>
+      if String.eqb x y then TySet y b pred
+      else TySet y b (expr_subst_surf x s pred)
+  | TyArr t1 t2 => TyArr (ty_subst_surf x s t1) (ty_subst_surf x s t2)
+  | TyArrDep y t1 t2 =>
+      if String.eqb x y then TyArrDep y (ty_subst_surf x s t1) t2
+      else TyArrDep y (ty_subst_surf x s t1) (ty_subst_surf x s t2)
+  | TyProd t1 t2 => TyProd (ty_subst_surf x s t1) (ty_subst_surf x s t2)
+  | TyRef t => TyRef (ty_subst_surf x s t)
+  | TyDeRef t => TyDeRef (ty_subst_surf x s t)
+  end.
