src/type_directed_translation.v
@@ -1,87 +1,13 @@
 Require Import DTDT.syntax.
-Require Import DTDT.big_step_eval.
-Require Import DTDT.semantic_rules.
+Require Import DTDT.big_step_eval_inter.
+Require Import DTDT.semantic_rules_inter.
+Require Import DTDT.semantic_rules_surf.
 
 (* --- Type directed translation from surface language to internal language -------------- *)
 
 Inductive mode : Type :=
   | sim : mode
   | dep : mode.
-
-(* --- Pure term validation - surface language -------------------------------------------- *)
-
-Fixpoint is_simple_type_surf (type : ty) : bool :=
-  match type with
-  | TyBase _ => true
-  | TyArr t1 t2 => is_simple_type_surf t1 && is_simple_type_surf t2
-  | TyProd t1 t2 => is_simple_type_surf t1 && is_simple_type_surf t2
-  | _ => false
-  end.
-
-Definition essential_type_is_base_type_surf (type : ty) : bool :=
-  match type with
-  | TyBase _ => true
-  | TySet _ _ _ => true
-  | _ => false
-  end.
-Notation "βs[ t ]" := (essential_type_is_base_type_surf t) (at level 10).
-
-Inductive has_type_pure_surf
-  ( Γ : var_context_surf)
-  (Φ : const_context_surf)
-  : expr -> ty -> Prop :=
-  | PVarS :
-    forall x τb,
-      Γs[ x ] Γ = Some τb ->
-      βs[ τb ] ->
-      has_type_pure_surf Γ Φ (ExVar x) τb
-  | PNatS :
-    forall n,
-      has_type_pure_surf Γ Φ (ExNat n) (TyBase BNat)
-  | PBoolS :
-    forall b,
-      has_type_pure_surf Γ Φ (ExBool b) (TyBase BBool)
-  | PStringS :
-    forall s,
-      has_type_pure_surf Γ Φ (ExString s) (TyBase BString)
-  | PUnitS :
-    forall u,
-      has_type_pure_surf Γ Φ (ExUnit u) (TyBase BUnit)
-  | PConstS :
-    forall c τ,
-      Φs[ c ] Φ = Some τ ->
-      is_simple_type_surf τ ->
-      has_type_pure_surf Γ Φ (ExConst c) τ
-  | PAppS :
-    forall e₁ e₂ τ₁ τ₂,
-      βs[ τ₁ ] ->
-      has_type_pure_surf Γ Φ e₁ (TyArr τ₁ τ₂) ->
-      has_type_pure_surf Γ Φ e₂ τ₁ ->
-      has_type_pure_surf Γ Φ (ExApp e₁ e₂) τ₂
-  | PNotS :
-    forall b,
-      has_type_pure_surf Γ Φ b (TyBase BBool) ->
-      has_type_pure_surf Γ Φ (ExNot b) (TyBase BBool)
-  | PImpS :
-    forall b₁ b₂,
-      has_type_pure_surf Γ Φ b₁ (TyBase BBool) ->
-      has_type_pure_surf Γ Φ b₂ (TyBase BBool) ->
-      has_type_pure_surf Γ Φ (ExImp b₁ b₂) (TyBase BBool)
-  | PAndS :
-    forall b₁ b₂,
-      has_type_pure_surf Γ Φ b₁ (TyBase BBool) ->
-      has_type_pure_surf Γ Φ b₂ (TyBase BBool) ->
-      has_type_pure_surf Γ Φ (ExAnd b₁ b₂) (TyBase BBool)
-  | POrS :
-    forall b₁ b₂,
-      has_type_pure_surf Γ Φ b₁ (TyBase BBool) ->
-      has_type_pure_surf Γ Φ b₂ (TyBase BBool) ->
-      has_type_pure_surf Γ Φ (ExOr b₁ b₂) (TyBase BBool)
-  | PPlusS :
-    forall n₁ n₂,
-      has_type_pure_surf Γ Φ n₁ (TyBase BNat) ->
-      has_type_pure_surf Γ Φ n₂ (TyBase BNat) ->
-      has_type_pure_surf Γ Φ (ExPlus n₁ n₂) (TyBase BNat).
 
 (* --- Translate surface type to internal type --------------------------------------- *)
 
@@ -127,21 +53,10 @@ with trans_expr (e : expr) : i_expr :=
   | EDep e => trans_expr e
   end.
 
-Definition trans_var_context_surf (Γs : var_context_surf) : var_context :=
-  map (fun p => (fst p, trans_type (snd p))) Γs.
-Notation "x >>ᵥ" := (trans_var_context_surf x) (at level 1).
-
-Definition trans_varval_context_surf (Γvs : varval_context_surf) : varval_context :=
-  map (fun p => (fst p, trans_expr (snd p))) Γvs.
-Notation "x >>ᵥᵥ" := (trans_varval_context_surf x) (at level 1).
-
-Definition trans_const_context_surf (Φs : const_context_surf) : const_context :=
-  map (fun p => (fst p, trans_type (snd p))) Φs.
-Notation "x >>φ" := (trans_const_context_surf x) (at level 1).
-
-Definition trans_fun_imp_list_surf (ιs : fun_imp_list_surf) : fun_imp_list :=
-  map (fun p => (fst p, trans_expr (snd p))) ιs.
-Notation "x >>ᵢ" := (trans_fun_imp_list_surf x) (at level 1).
+Definition trans_ctx_surf (Γs : ctx_surf) : ctx :=
+  (fmap (λ '(t, e), (trans_type t, trans_expr e)) (Γs ▷surfvars),
+   fmap (λ '(t, e), (trans_type t, trans_expr e)) (Γs ▷surfconsts)).
+Notation "x >>" := (trans_ctx_surf x) (at level 1).
 
 (* ------------------------------------------------------------------------- *)
 (* Erase dependency occurrences of a variable `x` from an internal type      *)
@@ -152,7 +67,7 @@ Fixpoint erase_dep_var (x : string) (τ : i_ty) : i_ty :=
   match τ with
   | TBase b => TBase b
   | TSet y b pred => if String.eqb x y then TSet y b pred else
-                      if in_dec string_dec x (exp_vars pred) then TBase b else TSet y b pred
+                      if existsb (String.eqb x) (exp_vars pred) then TBase b else TSet y b pred
   | TArr t1 t2 => TArr (erase_dep_var x t1) (erase_dep_var x t2)
   | TArrDep y t1 t2 => TArr (erase_dep_var x t1) (erase_dep_var x t2)
   | TProd t1 t2 => TProd (erase_dep_var x t1) (erase_dep_var x t2)
@@ -160,228 +75,283 @@ Fixpoint erase_dep_var (x : string) (τ : i_ty) : i_ty :=
   end.
 Notation "[[ t ]] x" := (erase_dep_var x t) (at level 1).
 
+(* --- Erase dependency in i_ty -------------------------------------------- *)
+
+Fixpoint erase_i_ty (τ : i_ty) : i_ty :=
+  match τ with
+  | TBase b =>
+      TBase b
+  | TSet x b _ =>
+      TSet x b (EBool true)
+  | TArr t1 t2 =>
+      TArr (erase_i_ty t1) (erase_i_ty t2)
+  | TArrDep _ t1 t2 =>
+      TArr (erase_i_ty t1) (erase_i_ty t2)
+  | TProd t1 t2 =>
+      TProd (erase_i_ty t1) (erase_i_ty t2)
+  | TRef t =>
+      TRef (erase_i_ty t)
+  end.
+Notation "[| t |]" := (erase_i_ty t) (at level 1).
+
 (* ------------------------------------------------------------------------- *)
 (* Type coercion judgment (internal language)                                *)
 (*   coerce ω Γ Γv Φ ι e τₛ e' τₜ  represents:                               *)
 (*     Γ Γv Φ ι ⊢ω e : τₛ → e' : τₜ                                          *)
 (* ------------------------------------------------------------------------- *)
 
-Inductive coerce (w : mode) (Γ : var_context) (Γv : varval_context) (Φ : const_context) (ι : fun_imp_list) :
+Inductive coerce (w : mode) (Γ : ctx) :
   i_expr -> i_ty -> i_expr -> i_ty -> Prop :=
   | CSub :
     forall e τ τ',
       (* when subtype holds no runtime conversion required *)
-      subtype Γ Γv Φ ι τ τ' ->
-      coerce w Γ Γv Φ ι
+      subtype Γ τ τ' ->
+      coerce w Γ
         e τ
         e τ'
   | CBase :
     forall e e₁ e₂ τ τb var,
       w = sim ->
-      τ = (TBase τb) \/ ty_valid Γ Φ (TSet var τb e₂) ->
-      coerce w Γ Γv Φ ι
-        e τ
+      τ = (TBase τb) \/ τ = (TSet var τb e₂) ->
+      coerce w Γ
+        e                                             τ
         (expr_subst var e (EIf e₁ (EVar var) EFail)) (TSet var τb e₁)
   | CFunCo :
-    forall e x τ₁ τ₂ τ₁' τ₂' y eᵦ,
+    forall e x τ₁ τ₂ τ₁' τ₂' y eᵦ v₁ v₂,
       w = sim ->
-      subtype Γ Γv Φ ι τ₁' τ₁ ->
-      coerce w ((y , TArrDep x τ₁ τ₂) :: (x, τ₁') :: Γ) Γv Φ ι
+      subtype Γ τ₁' τ₁ ->
+      coerce w (ctx_add_var (ctx_add_const Γ y (TArrDep x τ₁ τ₂) v₁) x τ₁' v₂)
         (EApp (EVar y) (EVar x)) τ₂
-        eᵦ τ₂' ->
-      coerce w Γ Γv Φ ι
-        e (TArr τ₁ τ₂)
+        eᵦ                       τ₂' ->
+      coerce w Γ
+        e                                                                     (TArr τ₁ τ₂)
         (expr_subst y e (EFix (fresh_string_list (exp_vars eᵦ)) x τ₁' τ₂' eᵦ)) (TArr τ₁' τ₂')
   | CFunContNonDep :
-    forall e eᵦ eₓ x y τ₁ τ₂ τ₁' τ₂',
+    forall e eᵦ eₓ x y τ₁ τ₂ τ₁' τ₂' v₁ v₂,
       w = sim ->
-      ~ subtype Γ Γv Φ ι τ₁' τ₁ ->
-      coerce w ((x , τ₁') :: Γ) Γv Φ ι
+      ~ subtype Γ τ₁' τ₁ ->
+      coerce w (ctx_add_var Γ x τ₁' v₁)
         (EVar x) τ₁'
-        eₓ τ₁ ->
-      coerce w ((y , TArr τ₁ τ₂) :: (x , τ₁') :: Γ) Γv Φ ι
+        eₓ       τ₁ ->
+      coerce w (ctx_add_var (ctx_add_const Γ y (TArrDep x τ₁ τ₂) v₁) x τ₁' v₂)
         (EApp (EVar y) eₓ) τ₂
-        eᵦ τ₂' ->
-      coerce w Γ Γv Φ ι
-        e (TArr τ₁ τ₂)
+        eᵦ                 τ₂' ->
+      coerce w Γ
+        e                                                                     (TArr τ₁ τ₂)
         (expr_subst y e (EFix (fresh_string_list (exp_vars eᵦ)) x τ₁' τ₂' eᵦ)) (TArr τ₁' τ₂')
   | CFunContDep :
-    forall e eᵦ eᵦ' e₁ e₁' x y τ₁ τ₂ τ₁' τ₂' τb,
+    forall e eᵦ eᵦ' e₁ e₁' x y τ₁ τ₂ τ₁' τ₂' τb v₁ v₂,
       w = sim ->
-      ~ subtype Γ Γv Φ ι τ₁' τ₁ ->
+      ~ subtype Γ τ₁' τ₁ ->
       τ₁ = TSet x τb e₁ ->
       τ₁' = TSet x τb e₁' \/ τ₁' = TBase τb ->
-      coerce w ((y , TArrDep x τ₁ τ₂) :: (x , τ₁) :: Γ) Γv Φ ι
+      coerce w (ctx_add_var (ctx_add_const Γ y (TArr τ₁ τ₂) v₂) x τ₁' v₁)
         (EApp (EVar y) (EVar x)) τ₂
-        eᵦ τ₂' ->
+        eᵦ                       τ₂' ->
       eᵦ' = EIf e₁ eᵦ EFail ->
-      coerce w Γ Γv Φ ι
-        e (TArrDep x τ₁ τ₂)
+      coerce w Γ
+        e                                                                       (TArrDep x τ₁ τ₂)
         (expr_subst y e (EFix (fresh_string_list (exp_vars eᵦ')) x τ₁' τ₂' eᵦ')) (TArrDep x τ₁' τ₂')
   | CPair :
-    forall e τ₁ τ₂ y e₁ e₂ τ₁' τ₂',
+    forall e τ₁ τ₂ y e₁ e₂ τ₁' τ₂' v,
       w = sim ->
-      coerce w ((y, TProd τ₁ τ₂) :: Γ) Γv Φ ι (EFst (EVar y)) τ₁ e₁ τ₁' ->
-      coerce w ((y, TProd τ₁ τ₂) :: Γ) Γv Φ ι (ESnd (EVar y)) τ₂ e₂ τ₂' ->
-      coerce w Γ Γv Φ ι e (TProd τ₁ τ₂)
-             (expr_subst y e (EPair e₁ e₂)) (TProd τ₁' τ₂')
+      coerce w (ctx_add_var Γ y (TProd τ₁ τ₂) v)
+        (EFst (EVar y)) τ₁
+        e₁              τ₁' ->
+      coerce w (ctx_add_var Γ y (TProd τ₁ τ₂) v)
+        (ESnd (EVar y)) τ₂
+        e₂              τ₂' ->
+      coerce w Γ
+        e                              (TProd τ₁ τ₂)
+        (expr_subst y e (EPair e₁ e₂)) (TProd τ₁' τ₂')
 .
 
-(* --- Type wellformedness for surface language -----------------------------*)
+(* --- Meet and join (τ₁ ⊓ τ₂ / τ₁ ⊔ τ₂) ----------------------------------- *)
 
-Inductive ty_valid_surf
-  (Γ : var_context_surf)
-  (Φ : const_context_surf)
-  : ty -> Prop :=
-  | VBaseS :
-    forall (τb : BaseT),
-      ty_valid_surf Γ Φ (TyBase τb)
-  | VSetS :
-    forall var (τb : BaseT) e,
-      has_type_pure_surf ((var , TyBase τb) :: Γ) Φ e (TyBase BBool) ->
-      ty_valid_surf Γ Φ (TySet var τb e)
-  | VFunS :
-    forall τ₁ τ₂,
-      ty_valid_surf Γ Φ τ₁ ->
-      ty_valid_surf Γ Φ τ₂ ->
-      ty_valid_surf Γ Φ (TyArr τ₁ τ₂)
-  | VFunDepS :
-    forall var τ₁ τ₂,
-      ty_valid_surf Γ Φ τ₁ ->
-      ty_valid_surf ((var, τ₁) :: Γ) Φ τ₂ ->
-      ty_valid_surf Γ Φ (TyArrDep var τ₁ τ₂)
-  | VPairS :
-    forall τ₁ τ₂,
-      ty_valid_surf Γ Φ τ₁ ->
-      ty_valid_surf Γ Φ τ₂ ->
-      ty_valid_surf Γ Φ (TyProd τ₁ τ₂)
-  | VRefS :
-    forall τ₁,
-      ty_valid_surf Γ Φ τ₁ ->
-      ty_valid_surf Γ Φ (TyRef τ₁)
-  | VDeRefS :
-    forall τ₁,
-      ty_valid_surf Γ Φ τ₁ ->
-      ty_valid_surf Γ Φ (TyDeRef τ₁).
+Inductive ty_meet (Γ : ctx) : i_ty -> i_ty -> i_ty -> Prop :=
+  | MeetBase :
+    forall b,
+      ty_meet Γ (TBase b) (TBase b) (TBase b)
+  | MeetSet :
+    forall x b e1 e2,
+      ty_meet Γ (TSet x b e1) (TSet x b e2) (TSet x b (EAnd e1 e2))
+  | MeetBaseLeft :
+    forall x b e,
+      ty_meet Γ (TBase b) (TSet x b e) (TSet x b e)
+  | MeetBaseRight :
+    forall x b e,
+      ty_meet Γ (TSet x b e) (TBase b) (TSet x b e)
+  | MeetArr :
+    forall τ1 τ1' τ2 τ2' dom cod,
+      ty_join Γ τ1 τ1' dom ->
+      ty_meet Γ τ2 τ2' cod ->
+      ty_meet Γ (TArr τ1 τ2) (TArr τ1' τ2') (TArr dom cod)
+  | MeetArrDep :
+    forall x τ1 τ1' τ2 τ2' dom cod v,
+      ty_join Γ τ1 τ1' dom ->
+      ty_meet (ctx_add_var Γ x τ1 v) τ2 τ2' cod ->
+      ty_meet Γ (TArrDep x τ1 τ2) (TArrDep x τ1' τ2') (TArrDep x dom cod)
+  | MeetProd :
+    forall τ1 τ1' τ2 τ2' m1 m2,
+      ty_meet Γ τ1 τ1' m1 ->
+      ty_meet Γ τ2 τ2' m2 ->
+      ty_meet Γ (TProd τ1 τ2) (TProd τ1' τ2') (TProd m1 m2)
+  | MeetRef :
+    forall τ τ' m,
+      ty_meet Γ τ τ' m ->
+      ty_meet Γ (TRef τ) (TRef τ') (TRef m)
+
+with ty_join (Γ : ctx) : i_ty -> i_ty -> i_ty -> Prop :=
+  | JoinBase :
+    forall b,
+      ty_join Γ (TBase b) (TBase b) (TBase b)
+  | JoinSet :
+    forall x b e1 e2,
+      ty_join Γ (TSet x b e1) (TSet x b e2) (TSet x b (EOr e1 e2))
+  | JoinBaseLeft :
+    forall x b e,
+      ty_join Γ (TBase b) (TSet x b e) (TSet x b e)
+  | JoinBaseRight :
+    forall x b e,
+      ty_join Γ (TSet x b e) (TBase b) (TSet x b e)
+  | JoinArr :
+    forall τ1 τ1' τ2 τ2' dom cod,
+      ty_meet Γ τ1 τ1' dom ->
+      ty_join Γ τ2 τ2' cod ->
+      ty_join Γ (TArr τ1 τ2) (TArr τ1' τ2') (TArr dom cod)
+  | JoinArrDep :
+    forall x τ1 τ1' τ2 τ2' dom cod v,
+      ty_meet Γ τ1 τ1' dom ->
+      ty_join (ctx_add_var Γ x dom v) τ2 τ2' cod ->
+      ty_join Γ (TArrDep x τ1 τ2) (TArrDep x τ1' τ2') (TArrDep x dom cod)
+  | JoinProd :
+    forall τ1 τ1' τ2 τ2' j1 j2,
+      ty_join Γ τ1 τ1' j1 ->
+      ty_join Γ τ2 τ2' j2 ->
+      ty_join Γ (TProd τ1 τ2) (TProd τ1' τ2') (TProd j1 j2)
+  | JoinRef :
+    forall τ τ' j,
+      ty_join Γ τ τ' j ->
+      ty_join Γ (TRef τ) (TRef τ') (TRef [| j |]).
 
 (* ------------------------------------------------------------------------- *)
 (* Surface language typing & translation judgment                            *)
 (*   has_type_surf w Γ Φ e e0 τ  corresponds to  ⊢^w e ; e0 : τ              *)
 (* ------------------------------------------------------------------------- *)
 
-Inductive has_type_surf (w : mode) (Γ : var_context_surf) (Γv : varval_context_surf) (Φ : const_context_surf) (ι : fun_imp_list_surf) :
+Inductive has_type_surf (w : mode) (Γ : ctx_surf) :
   expr -> i_expr -> i_ty -> Prop :=
   | ATNat :
     forall n,
-      has_type_surf w Γ Γv Φ ι (ExNat n) (ENat n) (TBase BNat)
+      has_type_surf w Γ (ExNat n) (ENat n) (TBase BNat)
   | ATBool :
     forall b,
-      has_type_surf w Γ Γv Φ ι (ExBool b) (EBool b) (TBase BBool)
+      has_type_surf w Γ (ExBool b) (EBool b) (TBase BBool)
   | ATString :
     forall s,
-      has_type_surf w Γ Γv Φ ι (ExString s) (EString s) (TBase BString)
+      has_type_surf w Γ (ExString s) (EString s) (TBase BString)
   | ATUnit :
     forall u,
-      has_type_surf w Γ Γv Φ ι (ExUnit u) (EUnit u) (TBase BUnit)
+      has_type_surf w Γ (ExUnit u) (EUnit u) (TBase BUnit)
   | ATConstSelf :
-    forall c τs,
-      Φs[ c ] Φ = Some τs ->
-      has_type_pure_surf Γ Φ (ExConst c) τs ->
-      has_type_surf w Γ Γv Φ ι (ExConst c) (EConst c) (self (trans_type τs) (EConst c))
+    forall c τs v,
+      Γ !!₂ₛ c = Some (τs, v) ->
+      has_type_pure_surf Γ (ExConst c) τs ->
+      has_type_surf w Γ (ExConst c) (EConst c) (self (trans_type τs) (EConst c))
   | ATConst :
-    forall c τs,
-      Φs[ c ] Φ = Some τs ->
-      ~ has_type_pure_surf Γ Φ (ExConst c) τs ->
-      has_type_surf w Γ Γv Φ ι (ExConst c) (EConst c) (trans_type τs)
+    forall c τs v,
+      Γ !!₂ₛ c = Some (τs, v) ->
+      ~ has_type_pure_surf Γ (ExConst c) τs ->
+      has_type_surf w Γ (ExConst c) (EConst c) (trans_type τs)
   | ATVarSelf :
-    forall x τs,
-      Γs[ x ] Γ = Some τs ->
-      has_type_pure_surf Γ Φ (ExVar x) τs ->
-      has_type_surf w Γ Γv Φ ι (ExVar x) (EVar x) (self (trans_type τs) (EVar x))
+    forall x τs v,
+      Γ !!₁ₛ x = Some (τs, v) ->
+      has_type_pure_surf Γ (ExVar x) τs ->
+      has_type_surf w Γ (ExVar x) (EVar x) (self (trans_type τs) (EVar x))
   | ATVar :
-    forall x τs,
-      Γs[ x ] Γ = Some τs ->
-      ~ has_type_pure_surf Γ Φ (ExVar x) τs ->
-      has_type_surf w Γ Γv Φ ι (ExVar x) (EVar x) (trans_type τs)
+    forall x τs v,
+      Γ !!₁ₛ x = Some (τs, v) ->
+      ~ has_type_pure_surf Γ (ExVar x) τs ->
+      has_type_surf w Γ (ExVar x) (EVar x) (trans_type τs)
   | ATFun :
-    forall f x τ₁ τ₂ τ₂' e e₁ e₂,
-      ty_valid_surf Γ Φ (TyArrDep x τ₁ τ₂) ->
-      has_type_surf w ((f , TyArrDep x τ₁ τ₂) :: (x , τ₁) :: Γ) Γv Φ ι e e₁ τ₂' ->
-      coerce w (((f , TyArrDep x τ₁ τ₂) :: (x , τ₁) :: Γ) >>ᵥ) (Γv >>ᵥᵥ) (Φ >>φ) (ι >>ᵢ)
+    forall f x τ₁ τ₂ τ₂' e e₁ e₂ v₁ v₂,
+      ty_valid_surf Γ (TyArrDep x τ₁ τ₂) ->
+      has_type_surf w (ctx_add_var_surf (ctx_add_const_surf Γ f (TyArrDep x τ₁ τ₂) v₂) x τ₁ v₁) e e₁ τ₂' ->
+      coerce w ((ctx_add_var_surf (ctx_add_const_surf Γ f (TyArrDep x τ₁ τ₂) v₂) x τ₁ v₁) >>)
         e₁ τ₂'
         e₂ (trans_type τ₂) ->
-      has_type_surf w Γ Γv Φ ι (ExFix f x τ₁ τ₂ e)
+      has_type_surf w Γ (ExFix f x τ₁ τ₂ e)
                     (EFix f x (trans_type τ₁) (trans_type τ₁) e₂)
                     (TArrDep x (trans_type τ₁) (trans_type τ₂))
   | ATAppPure :
     forall e₁ e₂ e₁' e₂' e₂'' x τ₁ τ₂ τ₁',
-      has_type_surf w Γ Γv Φ ι e₁ e₁' (TArrDep x τ₁ τ₂) ->
-      has_type_surf w Γ Γv Φ ι e₂ e₂' τ₁' ->
-      coerce w (Γ >>ᵥ) (Γv >>ᵥᵥ) (Φ >>φ) (ι >>ᵢ)
+      has_type_surf w Γ e₁ e₁' (TArrDep x τ₁ τ₂) ->
+      has_type_surf w Γ e₂ e₂' τ₁' ->
+      coerce w (Γ >>)
         e₂' τ₁'
         e₂'' τ₁ ->
-      (forall τ, has_type_pure (Γ >>ᵥ) (Φ >>φ) e₂'' τ) ->
-      has_type_surf w Γ Γv Φ ι (ExApp e₁ e₂) (EApp e₁' e₂'') (ty_subst x e₂'' τ₂)
+      (forall τ, has_type_pure (Γ >>) e₂'' τ) ->
+      has_type_surf w Γ (ExApp e₁ e₂) (EApp e₁' e₂'') (ty_subst x e₂'' τ₂)
   | ATAppImPure :
     forall e₁ e₂ e₁' e₁'' e₂' e₂'' x τ₁ τ₂ τ₁',
-      has_type_surf w Γ Γv Φ ι e₁ e₁' (TArrDep x τ₁ τ₂) ->
-      has_type_surf w Γ Γv Φ ι e₂ e₂' τ₁' ->
-      coerce w (Γ >>ᵥ) (Γv >>ᵥᵥ) (Φ >>φ) (ι >>ᵢ)
+      has_type_surf w Γ e₁ e₁' (TArrDep x τ₁ τ₂) ->
+      has_type_surf w Γ e₂ e₂' τ₁' ->
+      coerce w (Γ >>)
         e₂' τ₁'
         e₂'' τ₁ ->
-      ~ (forall τ, has_type_pure (Γ >>ᵥ) (Φ >>φ) e₂'' τ) ->
-      coerce w (Γ >>ᵥ) (Γv >>ᵥᵥ) (Φ >>φ) (ι >>ᵢ)
+      ~ (forall τ, has_type_pure (Γ >>) e₂'' τ) ->
+      coerce w (Γ >>)
         e₁' (TArrDep x τ₁ τ₂)
         e₁'' (TArr τ₁ ([[ τ₂ ]] x)) ->
-      has_type_surf w Γ Γv Φ ι (ExApp e₁ e₂) (EApp e₁'' e₂'') ([[ τ₂ ]] x)
+      has_type_surf w Γ (ExApp e₁ e₂) (EApp e₁'' e₂'') ([[ τ₂ ]] x)
   | ATProd :
     forall e₁ e₂ e₁' e₂' τ₁ τ₂,
-      has_type_surf w Γ Γv Φ ι e₁ e₁' τ₁ ->
-      has_type_surf w Γ Γv Φ ι e₂ e₂' τ₂ ->
-      has_type_surf w Γ Γv Φ ι (ExPair e₁ e₂) (EPair e₁' e₂') (TProd τ₁ τ₂)
+      has_type_surf w Γ e₁ e₁' τ₁ ->
+      has_type_surf w Γ e₂ e₂' τ₂ ->
+      has_type_surf w Γ (ExPair e₁ e₂) (EPair e₁' e₂') (TProd τ₁ τ₂)
   | ATFst :
     forall e e' τ₁ τ₂,
-      has_type_surf w Γ Γv Φ ι e e' (TProd τ₁ τ₂) ->
-      has_type_surf w Γ Γv Φ ι (ExFst e) (EFst e') τ₁
+      has_type_surf w Γ e e' (TProd τ₁ τ₂) ->
+      has_type_surf w Γ (ExFst e) (EFst e') τ₁
   | ATSnd :
     forall e e' τ₁ τ₂,
-      has_type_surf w Γ Γv Φ ι e e' (TProd τ₁ τ₂) ->
-      has_type_surf w Γ Γv Φ ι (ExSnd e) (ESnd e') τ₂
+      has_type_surf w Γ e e' (TProd τ₁ τ₂) ->
+      has_type_surf w Γ (ExSnd e) (ESnd e') τ₂
   | ATIfPure :
     forall e e₁ e₂ e₁' e₁'' e₂' e₂'' τ₁ τ₂ τ₃ u,
-      has_type_pure_surf Γ Φ e (TyBase BBool) ->
-      has_type_surf w ((u , TyBase BBool) :: Γ) ((u , e) :: Γv) Φ ι e₁ e₁' τ₁ ->
-      has_type_surf w ((u , TyBase BBool) :: Γ) ((u , ExNot e) :: Γv) Φ ι e₂ e₂' τ₂ ->
-      coerce w (((u , TyBase BBool) :: Γ) >>ᵥ) (((u , e) :: Γv) >>ᵥᵥ) (Φ >>φ) (ι >>ᵢ)
+      has_type_pure_surf Γ e (TyBase BBool) ->
+      has_type_surf w (ctx_add_var_surf Γ u (TyBase BBool) e) e₁ e₁' τ₁ ->
+      has_type_surf w (ctx_add_var_surf Γ u (TyBase BBool) (ExNot e)) e₂ e₂' τ₂ ->
+      coerce w ((ctx_add_var_surf Γ u (TyBase BBool) e) >>)
         e₁' τ₁
         e₁'' τ₃ ->
-      coerce w (((u , TyBase BBool) :: Γ) >>ᵥ) (((u , ExNot e) :: Γv) >>ᵥᵥ) (Φ >>φ) (ι >>ᵢ)
+      coerce w ((ctx_add_var_surf Γ u (TyBase BBool) (ExNot e)) >>)
         e₂' τ₂
         e₂'' τ₃ ->
-      (* TODO |_| definition *)
-      has_type_surf w Γ Γv Φ ι (ExIf e e₁ e₂) (EIf (trans_expr e) e₁'' e₂'') τ₃
+      ty_join (Γ >>) τ₁ τ₂ τ₃ ->
+      has_type_surf w Γ (ExIf e e₁ e₂) (EIf (trans_expr e) e₁'' e₂'') τ₃
   | ATIfImPure :
     forall e e₁ e₂ e' x τ,
-      ~ (forall τ', has_type_pure_surf Γ Φ e τ') ->
-      has_type_surf w Γ Γv Φ ι (* TODO kell surface subst is *)(ExIf (ExVar x) e₁ e₂) e' τ ->
-      has_type_surf w Γ Γv Φ ι (ExIf e e₁ e₂) e' τ
+      ~ (forall τ', has_type_pure_surf Γ e τ') ->
+      has_type_surf w Γ (expr_subst_surf x e (ExIf (ExVar x) e₁ e₂)) e' τ ->
+      has_type_surf w Γ (ExIf e e₁ e₂) e' τ
   (* TODO reference type rules *)
   | ATAssert :
     forall e e' e'' τ τ',
       w = dep ->
-      has_type_surf w Γ Γv Φ ι e e' τ' ->
-      ty_valid (Γ >>ᵥ) (Φ >>φ) (trans_type τ) ->
-      coerce sim (Γ >>ᵥ) (Γv >>ᵥᵥ) (Φ >>φ) (ι >>ᵢ)
+      has_type_surf w Γ e e' τ' ->
+      ty_valid (Γ >>) (trans_type τ) ->
+      coerce sim (Γ >>)
         e' τ'
         e'' (trans_type τ) ->
-      has_type_surf w Γ Γv Φ ι (EAssert e τ) e'' (trans_type τ)
+      has_type_surf w Γ (EAssert e τ) e'' (trans_type τ)
   | ATDynamic :
     forall e e' τ,
       w = dep ->
-      has_type_surf sim Γ Γv Φ ι e e' τ ->
-      has_type_surf w Γ Γv Φ ι (ESimple e) e' τ
+      has_type_surf sim Γ e e' τ ->
+      has_type_surf w Γ (ESimple e) e' τ
   | ATStatic :
     forall e e' τ,
       w = sim ->
-      has_type_surf dep Γ Γv Φ ι e e' τ ->
-      has_type_surf w Γ Γv Φ ι (EDep e) e' τ.
+      has_type_surf dep Γ e e' τ ->
+      has_type_surf w Γ (EDep e) e' τ.
